---
title: "36-402 Homework 5"
author:
- Eu Jing Chua
- eujingc
date: "February 19, 2019"
output:
  pdf_document: default
header-includes:
    - \usepackage{enumerate}
---

```{r setup, include=FALSE}
knitr::opts_chunk$set(echo = TRUE)
```

\newcommand{\est}[1]{\hat{#1}}
\newcommand{\betah}[1]{\est{\beta_{#1}}}
\newcommand{\avg}[1]{\overline{#1}}
\newcommand{\E}[1]{\mathbb{E} \left[ #1 \right]}
\newcommand{\Var}[1]{\text{Var} \left[ #1 \right]}
\newcommand{\Cov}[1]{\text{Cov} \left[ #1 \right]}
\newcommand{\X}{\mathbb{X}}
\newcommand{\sumTo}[1]{\sum^{#1}_{i=1}}
\newcommand{\sumjTo}[1]{\sum^{#1}_{j=1}}
\newcommand{\matr}[1]{\mathbf{#1}}
\newcommand{\txtsp}{\hspace{0.05in}}

# Question 1

**Q1 a)**

\begin{align}
\frac{1}{2h} \int_{x_0 - h}^{x_0 + h} (m + t(x - x_0) + c(x - x_0)^2) dx
    &= \frac{1}{2h} \int_{-h}^{h} (m + tu + cu^2) du, \txtsp u = x - x_0 \\
    &= \frac{1}{2h} \left[ mu + \frac{t}{2}u^2 + \frac{c}{3}u^3 \right]_{-h}^{h} \\
    &= \frac{1}{2h} (2mh + \frac{2}{3}ch^3) \\
    &= m + \frac{1}{3}ch^2 \\
    &\implies k = \frac{1}{3}
\end{align}

**Q1 b)**

\begin{align}
\E{m(X)} &= \int_{x_0 - h}^{x_0 + h} m(x) \frac{1}{2h} dx \\
    &= \frac{1}{2h} \int_{x_0 - h}^{x_0 + h} m(x) dx \\
    &\approx \frac{1}{2h} \int_{x_0 - h}^{x_0 + h} m(x_0) + m'(x_0) (x - x_0) + \frac{1}{2} m''(x_0)(x - x_0)^2 dx \\
    &= m(x_0) + \frac{m''(x_0)}{3} h^2
\end{align}

**Q1 c)**
Let $A_{x_0} = \{ i: |X_i - x_0| \le h \}$, so $\est{\mu}(x_0) = \frac{1}{|A_{x_0}|}\sum_{i \in A_{x_0}} Y_i$
\begin{align}
    \E{\est{\mu}(x_0)} &= \E{\frac{1}{|A_{x_0}|}\sum_{i \in A_{x_0}} Y_i} \\
        &= \E{\frac{1}{|A_{x_0}|}\sum_{i \in A_{x_0}} \mu(X_i) + \epsilon_i} \\
        &= \frac{1}{|A_{x_0}|}\sum_{i \in A_{x_0}} \E{\mu(X_i)} + \E{\epsilon_i} \\
        &= \E{\mu(X) \mid |X - x_0| \le h} + \E{\epsilon \mid |X - x_0| \le h} \\
        &\approx \mu(x_0) + \frac{\mu''(x_0)}{3} h^2 + 0 \\
        &= \mu(x_0) + O(h^2) \\
    \text{Bias}[\est{\mu}(x_0)] &= \E{\est{\mu}(x_0)} - \est{\mu}(x_0) \\
        &= O(h^2)
\end{align}

**Q1 d)**
\begin{align}
\E{m(X)} &= \int_{x_0 - h}^{x_0 + h} m(x) f(x) dx \\
    &\approx \int_{x_0 - h}^{x_0 + h} \left( m(x_0) + m'(x_0)(x - x_0) + \frac{1}{2} m''(x_0)(x - x_0)^2 \right) \left(f(x_0) + f'(x_0)(x - x_0) + \frac{1}{2} f''(x_0)(x - x_0)^2 \right) dx \\
    &\approx \int_{x_0 - h}^{x_0 + h} \left( m(x_0) f(x_0) + \left(\frac{1}{2} m(x_0)f''(x_0) + m'(x_0)f'(x_0) + \frac{1}{2} m''(x_0) f(x_0) \right) (x - x_0)^2 \right) dx \\
    &= m(x_0) f(x_0) + \frac{\frac{1}{2} m(x_0)f''(x_0) + m'(x_0)f'(x_0) + \frac{1}{2} m''(x_0) f(x_0)}{3} h^2
\end{align}
